src/lib/kernel/Kuiper.Kernel.LogSoftmax.fsti
@@ -7,33 +7,9 @@ open Kuiper.Seq.Common
 module Vec = Pulse.Lib.Vec
 module SM = Kuiper.Kernel.Softmax
 
-// Unfortunate to have to define and use this
-let seq_refine #a (p : a -> prop)
-  (s : seq a { forall i. p (s @! i) })
-  : GTot (lseq (x:a{p x}) (Seq.length s))
-  = Seq.init_ghost #(x:a{p x}) (Seq.length s) (fun i -> s @! i)
-
-let seq_refine_len #a (p : a -> prop)
-  (s : seq a { forall i. p (s @! i) })
-  : Lemma (len (seq_refine p s) == len s)
-          [SMTPat (Seq.length (seq_refine p s))]
-  = ()
-
-let seq_refine_at #a (p : a -> prop)
-  (s : seq a { forall i. p (s @! i) })
-  (i : natlt (Seq.length s))
-  : Lemma ((seq_refine p s) @! i == s @! i)
-          [SMTPat ((seq_refine p s) @! i)]
-  = ()
-
 // Log of softmax.
 let log_softmax_real (s:Seq.seq real { Seq.length s > 0 }) =
   lseq_map rlog (seq_refine (fun x -> x >. 0.0R) (SM.softmax_real s))
-
-let log_softmax_real' (s:Seq.seq real { Seq.length s > 0 }) =
-  let exps = seq_map rexp s in
-  let summ : real = SM.sum exps in
-  lseq_map #_ #_ #(Seq.length s) FStar.Real.(fun x -> x -. rlog summ) s
 
 unfold
 type log_softmax_ty (et : Type0) {| floating et, real_like et |} =
@@ -54,4 +30,4 @@ type log_softmax_ty (et : Type0) {| floating et, real_like et |} =
 
 inline_for_extraction noextract
 val log_softmax (#et : Type0) {| floating et, real_like et, floating_real_like et |}
-: log_softmax_ty et
+  : log_softmax_ty et
