src/lib/kernel/Kuiper.Kernel.Softmax.fst
@@ -18,89 +18,17 @@ open Kuiper.Array1
 open Kuiper.Tensor { ctlayout }
 open Kuiper.Tensor.Layout.Alg { l1_forward }
 
-(* From the CPU, read one element from a flat array1. *)
-inline_for_extraction noextract
-fn arr_read_1
-  (#et : Type0) {| sized et |}
-  (#len : erased nat)
-  (a : Array1.t et (l1_forward len))
-  (i : szlt len)
-  (#f : perm)
-  (#va : erased (lseq et len))
-  preserves
-    cpu
-  preserves
-    on gpu_loc (a |-> Frac f va)
-  returns
-    x : et
-  ensures
-    pure (x == va @! i)
-{
-  let ca = Pulse.Lib.Vec.alloc #et default 1sz;
-
-  map_loc gpu_loc
-    #(a |-> Frac f va)
-    #(core a |-> Frac f va)
-    fn _ {
-      Array1.lower a;
-      assert pure (Seq.equal (to_seq (l1_forward len) va) va);
-      rewrite core a |-> Frac f (to_seq (l1_forward len) va)
-           as core a |-> Frac f va;
-    };
-
-  (* FIXME: Need to give length of ca?!? *)
-  gpu_memcpy_device_to_host' #_ #_ #1 ca 0sz (core a) i 1sz;
-
-  let x = Pulse.Lib.Vec.(ca.(0sz));
-  Pulse.Lib.Vec.free ca;
-
-  map_loc gpu_loc
-    #(core a |-> Frac f va)
-    #(a |-> Frac f va)
-    fn _ {
-      Array1.raise' (l1_forward len) (core a);
-      rewrite each from_array (l1_forward len) (core a) as a;
-      assert pure (Seq.equal (from_seq (l1_forward len) va) va);
-      ();
-    };
-
-  x;
-}
-
-let map_div_avg (#et:Type0) {| floating et |} (s:Seq.seq et) (avg:et) =
-  let exps = seq_map exp s in
-  seq_map (fun x -> div x avg) s
-
-let softmax_spec (#et:Type0) {| floating et |} (s:Seq.seq et) =
-  let exps = seq_map exp s in
-  let avg = seq_fold_left add zero exps in
-  map_div_avg exps avg
-
-let rec sum_non_zero
-    (s:seq real { forall (i:natlt (Seq.length s)). Seq.index s i >. 0.0R })
-    (acc:real)
-: Lemma
-  (requires Seq.length s > 0)
-  (ensures  seq_fold_left add acc s >. acc)
-  (decreases Seq.length s)
-= if Seq.length s = 1 then ()
-  else
-    let SCons hd tl = view_seq s in
-    sum_non_zero tl (add acc hd <: real)
-
 let softmax_approx
     (#et:Type0) {| floating et, real_like et, floating_real_like et |}
     (s0:seq et) (r0:seq real { s0 %~ r0 /\ Seq.length r0 > 0 })
-    (summ : et)
-: Lemma
-  (ensures
-      summ %~ sum (seq_map rexp r0) ==>
-      seq_map (fun x -> div x summ) (seq_map exp s0) %~ softmax_real r0)
-= let exps = seq_map rexp r0 in
-  sum_non_zero exps 0.0R;
-  Classical.forall_intro_2 (fun x -> Classical.move_requires (exp_approx #et x));
-  Classical.forall_intro_4 (fun (x y : et) (r : real) -> Classical.move_requires (div_approx #et x y r));
-  ()
+    (summ : et{summ %~ rsum (seq_map rexp r0)})
+  : Lemma
+    (ensures seq_map (fun x -> div x summ) (seq_map exp s0) %~ softmax_real r0)
+  = let exps = seq_map rexp r0 in
+    sum_non_zero exps 0.0R;
+    Classical.forall_intro_2 (fun x -> Classical.move_requires (exp_approx #et x));
+    Classical.forall_intro_4 (fun (x y : et) (r : real) -> Classical.move_requires (div_approx #et x y r));
+    ()
 
 inline_for_extraction noextract
 fn softmax_gpu
